proof/agp32_IF_CorrectScript.sml
@@ -230,29 +230,6 @@ QED
 
 (** IF_instr updated when IF is disabled **)
 (** lemma **)
-Theorem same_t_and_m_under_MAX_SET_0[local]:
-  !fext t m.
-    MAX_SET {t0 | t0 < t /\ (fext t0).ready} = 0 ==>
-    (!p. p < m ==> ~(fext (p + 1)).ready) ==>
-    (fext (m + 1)).ready ==>
-    ~(fext t).ready ==>
-    (fext (t + 1)).ready ==>
-    m = t
-Proof
-  rw [] >> Cases_on `m = t` >> rw [] >>
-  Cases_on `t < m` >-
-   METIS_TAC [] >>
-  `t > m` by fs [] >> fs [] >>
-  Cases_on `t = m + 1` >> fs [] >>
-  `t > m + 1` by fs [] >>
-  `{t0 | t0 < t /\ (fext t0).ready} (m + 1)` by fs [] >>
-  Cases_on `{t0 | t0 < t /\ (fext t0).ready} = {}` >-
-   METIS_TAC [EMPTY_applied] >>
-  `FINITE {t0 | t0 < t /\ (fext t0).ready}` by rw [FINITE_max_ready_cycle] >>
-  `(m + 1) IN {t0 | t0 < t /\ (fext t0).ready}` by fs [] >>
-  `m + 1 <= 0` by METIS_TAC [MAX_SET_DEF] >> rw []
-QED
-
 Theorem PC_unchanged_after_disabled_cycles[local]:
   !fext fbits m n.
     (!p. p < m ==> ~(fext (p + n)).ready) ==>
@@ -275,23 +252,6 @@ Proof
       by METIS_TAC [agp32_same_IF_items_until_ID_pipeline,Abbr `s1`,Abbr `s2`] >>
     fs [IF_PC_update_def]) >>
   `n + SUC m = SUC (n + m)` by rw [] >> rw [] >> fs []
-QED
-
-Theorem not_ready_m_plus_n[local]:
-  !fext m n.
-    (!p. p < n ==> ~(fext (p + 1)).ready) ==>
-    (!p. p < m ==> ~(fext (n + (p + 1))).ready) ==>
-    (!p. p < m + n ==> ~(fext (p + 1)).ready)
-Proof
-  rw [] >>
-  Cases_on `p < n` >> fs [] >>
-  Cases_on `p = n` >> fs [] >-
-   (`~(fext (n + (0 + 1))).ready` by fs [] >>
-    `n + (0 + 1) = n + 1` by rw [] >> fs []) >>
-  `p > n` by fs [] >> fs [] >>
-  `p - n < m` by rw [] >>
-  `~(fext (n + (p - n + 1))).ready` by fs [] >>
-  `n + (p - n + 1) = p + 1` by rw [] >> fs []
 QED
 
 (** not ready at the previous cycle **)
