proof/agp32_MEM_Data_CorrectScript.sml
@@ -78,6 +78,58 @@ Proof
   `t0 + 1 <= 0` by METIS_TAC [MAX_SET_DEF] >> rw []
 QED
 
+Theorem same_mem_t_SUC_t_under_MAX_SET[local]:
+  !fext t m n.
+    MAX_SET {t0 | t0 < t /\ (fext t0).ready} = n ==>
+    (!p. p < m ==> ~(fext (p + (SUC n))).ready /\ (fext (p + SUC n)).mem = (fext n).mem) ==>
+    (fext (m + SUC n)).ready ==>
+    ~(fext t).ready ==>
+    ~(fext (SUC t)).ready ==>
+    n <> 0 ==>
+    (fext t).mem = (fext (SUC t)).mem
+Proof
+  rpt strip_tac >>
+  `FINITE {t0 | t0 < t /\ (fext t0).ready}` by fs [FINITE_max_ready_cycle] >>
+  Cases_on `{t0 | t0 < t /\ (fext t0).ready} = {}` >> fs [MAX_SET_DEF] >>
+  `n IN {t0 | t0 < t /\ (fext t0).ready}` by METIS_TAC [MAX_SET_DEF] >>
+  fs [MAX_SET_DEF] >>
+  Cases_on `m + SUC n = SUC t` >> fs [] >>
+  Cases_on `SUC t > m + SUC n` >-
+   (Cases_on `t = m + SUC n` >> fs [] >>
+    Cases_on `t > m + SUC n` >>
+    (`(m + SUC n) IN {t0 | t0 < t /\ (fext t0).ready}` by fs [] >>
+     `(m + SUC n) <= n` by METIS_TAC [MAX_SET_DEF] >> fs []) >> fs []) >>
+  `SUC t < m + SUC n /\ t < m + SUC n` by fs [] >>
+  `SUC t -SUC n < m /\ t - SUC n < m` by rw [] >>   
+  `(fext (SUC t -SUC n + SUC n)).mem = (fext n).mem /\
+  (fext (t -SUC n + SUC n)).mem = (fext n).mem` by fs [] >>
+  `SUC t -SUC n + SUC n = SUC t /\ t - SUC n + SUC n = t` by rw [] >> METIS_TAC []
+QED
+
+Theorem same_mem_t_SUC_t_under_MAX_SET_0[local]:
+  !fext t m n.
+    MAX_SET {t0 | t0 < t /\ (fext t0).ready} = 0 ==>
+    (!p. p < m ==> ~(fext (p + 1)).ready /\ (fext 0).mem = (fext (p + 1)).mem) ==>
+    (fext (m + 1)).ready ==>
+    ~(fext t).ready ==>
+    ~(fext (SUC t)).ready ==>
+    (fext t).mem = (fext (SUC t)).mem
+Proof
+  rw [ADD1] >> Cases_on `m = t` >> fs [] >>
+  Cases_on `t > m` >-
+   (Cases_on `t = m + 1` >> fs [] >>
+    `{t0 | t0 < t /\ (fext t0).ready} (m + 1)` by fs [] >>
+    Cases_on `{t0 | t0 < t /\ (fext t0).ready} = {}` >-
+     METIS_TAC [EMPTY_applied] >>
+    `FINITE {t0 | t0 < t /\ (fext t0).ready}` by rw [FINITE_max_ready_cycle] >>
+    `(m + 1) IN {t0 | t0 < t /\ (fext t0).ready}` by fs [] >>
+    `m + 1 <= 0` by METIS_TAC [MAX_SET_DEF] >> fs []) >>
+  `t < m` by fs [] >>
+  `t - 1 < m` by fs [] >>   
+  `(fext (t + 1)).mem = (fext 0).mem /\ (fext (t - 1 + 1)).mem = (fext 0).mem` by fs [] >>
+  Cases_on `t` >> fs [ADD1]
+QED
+
 
 (** memory **)
 (** WB **)
@@ -440,6 +492,7 @@ Proof
   METIS_TAC [agp32_Rel_ag32_fext_MEM_correct_WB_not_NONE_WB_disable_fext_not_ready]
 QED
 
+(** WB is not NONE and fext is ready **)
 Theorem agp32_Rel_ag32_fext_MEM_correct_WB_not_NONE:
   !fext fbits a t I.
     is_mem fext_accessor_circuit (agp32 fext fbits) fext ==>
@@ -452,6 +505,506 @@ Proof
   rw [] >> Cases_on `enable_stg 5 (agp32 fext fbits t)` >-
    METIS_TAC [agp32_Rel_ag32_fext_MEM_correct_WB_not_NONE_WB_enable] >>
   METIS_TAC [agp32_Rel_ag32_fext_MEM_correct_WB_not_NONE_WB_disable]
+QED
+
+
+(** WB enabled **)
+Theorem agp32_Rel_ag32_fext_MEM_correct_WB_not_NONE_WB_enable_extra:
+  !fext fbits a t I.
+    is_mem fext_accessor_circuit (agp32 fext fbits) fext ==>
+    is_sch I (agp32 fext fbits) a ==>
+    Rel I (fext t) (agp32 fext fbits (t-1)) (agp32 fext fbits t) a t ==>
+    I (5,SUC t) <> NONE ==>
+    ~(fext (SUC t)).ready ==>
+    enable_stg 5 (agp32 fext fbits t) ==>
+    (fext (SUC t)).mem = (FUNPOW Next (THE (I (5,SUC t)) - 1) a).MEM
+Proof
+  rw [] >> `I' (5,SUC t) = I' (4,t)` by fs [is_sch_def,is_sch_writeback_def] >>
+  `(fext t).ready` by (fs [enable_stg_def] >> METIS_TAC [agp32_WB_state_flag_and_fext_ready]) >>
+  Cases_on `I' (5,t) <> NONE` >> fs [] >-
+   (Cases_on `~is_wrMEM_isa (FUNPOW Next (THE (I' (4,t)) - 1) a)` >-
+     (fs [GSYM MEM_not_changed_after_normal_instrs] >>
+      last_assum (assume_tac o is_mem_def_mem_no_errors) >>
+      Cases_on_word_value `(agp32 fext fbits (SUC t)).command` >>
+      fs [agp32_command_impossible_values] >-
+       (last_assum (mp_tac o is_mem_data_flush `SUC t`) >> rw [] >>
+        Cases_on `m` >> fs [] >>
+        `(fext (0 + SUC t)).mem = (fext t).mem` by fs [] >> fs [] >>
+        `THE (I' (4,t)) = THE (I' (5,t)) + 1`
+            by METIS_TAC [MEM_instr_index_with_WB_instr_plus_1] >> fs [Rel_def]) >-
+       (fs [is_wrMEM_isa_def] >>
+        `(agp32 fext fbits t).MEM.MEM_opc <> 2w /\
+        (agp32 fext fbits t).MEM.MEM_opc <> 3w` by fs [Rel_def,MEM_Rel_def] >>
+        METIS_TAC [agp32_Rel_ag32_command_not_3_not_write_mem_and_byte_WB_enable]) >-
+       (last_assum (mp_tac o is_mem_data_read `SUC t`) >> rw [] >>
+        Cases_on `m` >> fs [] >>
+        `(fext (0 + SUC t)).mem = (fext t).mem` by fs [] >> fs [] >>
+        `THE (I' (4,t)) = THE (I' (5,t)) + 1`
+            by METIS_TAC [MEM_instr_index_with_WB_instr_plus_1] >> fs [Rel_def]) >-
+       (last_assum (mp_tac o is_mem_inst_read `SUC t`) >> rw [] >>
+        Cases_on `m` >> fs [] >>
+        `(fext (0 + SUC t)).mem = (fext t).mem` by fs [] >> fs [] >>
+        `THE (I' (4,t)) = THE (I' (5,t)) + 1`
+            by METIS_TAC [MEM_instr_index_with_WB_instr_plus_1] >> fs [Rel_def]) >>
+      last_assum (mp_tac o is_mem_do_nothing `SUC t`) >> rw []) >>
+    fs [is_wrMEM_isa_def] >-
+     (`(agp32 fext fbits t).MEM.MEM_opc = 2w` by fs [is_wrMEM_isa_def,Rel_def,MEM_Rel_def] >>
+      `(agp32 fext fbits (SUC t)).WB.WB_opc = 2w` by fs [agp32_WB_opc_MEM_opc_when_WB_enabled] >>
+      `(agp32 fext fbits (SUC t)).command = 3w`
+        by fs [agp32_Rel_ag32_command_correct_write_mem_WB_enable] >>
+      last_assum (mp_tac o is_mem_data_write `SUC t`) >> rw [] >>
+      Cases_on `m` >> fs [] >>
+      `(fext (0 + SUC t)).mem = (fext t).mem` by fs [] >> fs [] >>
+      `THE (I' (4,t)) = THE (I' (5,t)) + 1`
+        by METIS_TAC [MEM_instr_index_with_WB_instr_plus_1] >> fs [Rel_def]) >>
+    `(agp32 fext fbits t).MEM.MEM_opc = 3w` by fs [is_wrMEM_isa_def,Rel_def,MEM_Rel_def] >>
+    `(agp32 fext fbits (SUC t)).WB.WB_opc = 3w` by fs [agp32_WB_opc_MEM_opc_when_WB_enabled] >>
+    `(agp32 fext fbits (SUC t)).command = 3w`
+      by fs [agp32_Rel_ag32_command_correct_write_mem_byte_WB_enable] >>
+    last_assum (mp_tac o is_mem_data_write `SUC t`) >> rw [] >>
+    Cases_on `m` >> fs [] >>
+    `(fext (0 + SUC t)).mem = (fext t).mem` by fs [] >> fs [] >>
+    `THE (I' (4,t)) = THE (I' (5,t)) + 1`
+      by METIS_TAC [MEM_instr_index_with_WB_instr_plus_1] >> fs [Rel_def]) >>
+  Cases_on `~is_wrMEM_isa (FUNPOW Next (THE (I' (4,t)) - 1) a)` >-
+   (fs [GSYM MEM_not_changed_after_normal_instrs] >>
+    last_assum (assume_tac o is_mem_def_mem_no_errors) >>
+    Cases_on_word_value `(agp32 fext fbits (SUC t)).command` >>
+    fs [agp32_command_impossible_values] >-
+     (last_assum (mp_tac o is_mem_data_flush `SUC t`) >> rw [] >>
+      Cases_on `m` >> fs [] >>
+      `(fext (0 + SUC t)).mem = (fext t).mem` by fs [] >> fs [Rel_def]) >- 
+     (fs [is_wrMEM_isa_def] >>
+      `(agp32 fext fbits t).MEM.MEM_opc <> 2w /\
+      (agp32 fext fbits t).MEM.MEM_opc <> 3w` by fs [Rel_def,MEM_Rel_def] >>
+      METIS_TAC [agp32_Rel_ag32_command_not_3_not_write_mem_and_byte_WB_enable]) >- 
+     (last_assum (mp_tac o is_mem_data_read `SUC t`) >> rw [] >>
+      Cases_on `m` >> fs [] >>
+      `(fext (0 + SUC t)).mem = (fext t).mem` by fs [] >> fs [Rel_def]) >-
+     (last_assum (mp_tac o is_mem_inst_read `SUC t`) >> rw [] >>
+      Cases_on `m` >> fs [] >>
+      `(fext (0 + SUC t)).mem = (fext t).mem` by fs [] >> fs [Rel_def]) >>
+    last_assum (mp_tac o is_mem_do_nothing `SUC t`) >> rw []) >>
+  fs [is_wrMEM_isa_def] >-
+   (`(agp32 fext fbits t).MEM.MEM_opc = 2w` by fs [is_wrMEM_isa_def,Rel_def,MEM_Rel_def] >>
+    `(agp32 fext fbits (SUC t)).WB.WB_opc = 2w` by fs [agp32_WB_opc_MEM_opc_when_WB_enabled] >>
+    `(agp32 fext fbits (SUC t)).command = 3w`
+      by fs [agp32_Rel_ag32_command_correct_write_mem_WB_enable] >>
+    last_assum (mp_tac o is_mem_data_write `SUC t`) >> rw [] >>
+    Cases_on `m` >> fs [] >>
+    `(fext (0 + SUC t)).mem = (fext t).mem` by fs [] >> fs [Rel_def]) >>
+  `(agp32 fext fbits t).MEM.MEM_opc = 3w` by fs [is_wrMEM_isa_def,Rel_def,MEM_Rel_def] >>
+  `(agp32 fext fbits (SUC t)).WB.WB_opc = 3w` by fs [agp32_WB_opc_MEM_opc_when_WB_enabled] >>
+  `(agp32 fext fbits (SUC t)).command = 3w`
+    by fs [agp32_Rel_ag32_command_correct_write_mem_byte_WB_enable] >>
+  last_assum (mp_tac o is_mem_data_write `SUC t`) >> rw [] >>
+  Cases_on `m` >> fs [] >>       
+  `(fext (0 + SUC t)).mem = (fext t).mem` by fs [] >> fs [Rel_def]
+QED
+
+(** WB disabled and the previous cycle is not ready **)
+Theorem agp32_Rel_ag32_fext_MEM_correct_WB_not_NONE_WB_disable_fext_not_ready_extra:
+  !fext fbits a t I.
+    is_mem fext_accessor_circuit (agp32 fext fbits) fext ==>
+    is_sch I (agp32 fext fbits) a ==>
+    Rel I (fext t) (agp32 fext fbits (t-1)) (agp32 fext fbits t) a t ==>
+    I (5,SUC t) <> NONE ==>
+    ~(fext (SUC t)).ready ==>
+    ~(fext t).ready ==>
+    ~enable_stg 5 (agp32 fext fbits t) ==>
+    (fext (SUC t)).mem = (FUNPOW Next (THE (I (5,SUC t)) - 1) a).MEM
+Proof
+  rw [] >>
+  `(agp32 fext fbits (SUC t)).WB.WB_opc <> 16w` by METIS_TAC [WB_instr_index_not_NONE_opc_not_16] >>
+  Cases_on `MAX_SET {t0 | t0 < t /\ (fext t0).ready}` >-
+   (Cases_on `{t0 | t0 < t /\ (fext t0).ready} = {}` >-
+     (`!t0. t0 < t ==> ~(fext t0).ready` by METIS_TAC [EMPTY_no_fext_ready_cycle] >>
+      `(agp32 fext fbits t).WB.WB_opc = (agp32 fext fbits 0).WB.WB_opc`
+        by fs [WB_opc_unchanged_after_disabled_cycles_0] >>
+      gs [agp32_WB_opc_unchanged_when_WB_disabled,agp32_init_WB_opc]) >>
+    `!t0. t0 < t - 1 ==> ~(fext (t0 + 1)).ready`
+      by METIS_TAC [MAX_SET_0_no_fext_ready_cycle] >>
+    `(agp32 fext fbits (t - 1 + 1)).WB.WB_opc = (agp32 fext fbits 1).WB.WB_opc`
+      by fs [WB_opc_unchanged_after_disabled_cycles] >>
+    `t - 1 + 1 = t` by (Cases_on `t` >> fs []) >> fs [] >>
+    `(agp32 fext fbits t).WB.WB_opc <> 16w` by gs [agp32_WB_opc_unchanged_when_WB_disabled] >>
+    `~enable_stg 5 (agp32 fext fbits 0)` by fs [agp32_init_ctrl_flags,enable_stg_def] >>
+    `(agp32 fext fbits (SUC 0)).WB.WB_opc = 16w`
+      by fs [agp32_WB_opc_unchanged_when_WB_disabled,agp32_init_WB_opc] >>
+    fs [SUC_ONE_ADD]) >>
+  Q.ABBREV_TAC `i = SUC n` >> `i <> 0` by fs [Abbr `i`] >>
+  `FINITE {t0 | t0 < t /\ (fext t0).ready}` by fs [FINITE_max_ready_cycle] >>
+  Cases_on `{t0 | t0 < t /\ (fext t0).ready} = {}` >> fs [MAX_SET_DEF] >>
+  `i IN {t0 | t0 < t /\ (fext t0).ready}` by METIS_TAC [MAX_SET_DEF] >> fs [MAX_SET_DEF] >>
+  last_assum (assume_tac o is_mem_def_mem_no_errors) >>
+  Cases_on_word_value `(agp32 fext fbits (SUC i)).command` >>
+  fs [agp32_command_impossible_values] >-
+   (last_assum (mp_tac o is_mem_data_flush `SUC i`) >> simp [] >> strip_tac >>
+    `(fext (SUC t)).mem = (fext t).mem` by METIS_TAC [same_mem_t_SUC_t_under_MAX_SET] >>
+    gs [is_sch_def,is_sch_disable_def,Rel_def]) >-
+   (last_assum (mp_tac o is_mem_data_write `SUC i`) >> simp [] >> strip_tac >>
+    `(fext (SUC t)).mem = (fext t).mem` by METIS_TAC [same_mem_t_SUC_t_under_MAX_SET] >>
+    gs [is_sch_def,is_sch_disable_def,Rel_def]) >-
+   (last_assum (mp_tac o is_mem_data_read `SUC i`) >> simp [] >> strip_tac >>
+    `(fext (SUC t)).mem = (fext t).mem` by METIS_TAC [same_mem_t_SUC_t_under_MAX_SET] >>
+    gs [is_sch_def,is_sch_disable_def,Rel_def]) >-
+   (last_assum (mp_tac o is_mem_inst_read `SUC i`) >> simp [] >> strip_tac >>
+    `(fext (SUC t)).mem = (fext t).mem` by METIS_TAC [same_mem_t_SUC_t_under_MAX_SET] >>
+    gs [is_sch_def,is_sch_disable_def,Rel_def]) >>
+  last_assum (mp_tac o is_mem_do_nothing `SUC i`) >> simp [] >> strip_tac >>
+  Cases_on `SUC i = t` >> fs [] >>
+  Cases_on `SUC i > t` >> fs [] >>
+  `SUC i < t` by fs [] >>
+  `(SUC i) IN {t0 | t0 < t /\ (fext t0).ready}` by fs [] >>
+  `(SUC i) <= i` by METIS_TAC [MAX_SET_DEF] >> fs []
+QED
+
+(** WB disabled **)
+Theorem agp32_Rel_ag32_fext_MEM_correct_WB_not_NONE_WB_disable_extra:
+  !fext fbits a t I.
+    is_mem fext_accessor_circuit (agp32 fext fbits) fext ==>
+    is_sch I (agp32 fext fbits) a ==>
+    Rel I (fext t) (agp32 fext fbits (t-1)) (agp32 fext fbits t) a t ==>
+    I (5,SUC t) <> NONE ==>
+    ~(fext (SUC t)).ready ==>
+    ~enable_stg 5 (agp32 fext fbits t) ==>
+    (fext (SUC t)).mem = (FUNPOW Next (THE (I (5,SUC t)) - 1) a).MEM
+Proof
+  rw [] >> Cases_on `(fext t).ready` >-
+   (`I' (5,SUC t) = I' (5,t)` by fs [is_sch_def,is_sch_disable_def] >>
+    `(agp32 fext fbits (SUC t)).WB.WB_opc <> 16w` by METIS_TAC [WB_instr_index_not_NONE_opc_not_16] >>
+    `(agp32 fext fbits (SUC t)).WB.WB_opc = (agp32 fext fbits t).WB.WB_opc`
+      by fs [agp32_WB_opc_unchanged_when_WB_disabled] >>
+    last_assum (assume_tac o is_mem_def_mem_no_errors) >>
+    `(agp32 fext fbits (SUC t)).command = 0w`
+      by gs [agp32_Rel_ag32_command_correct_WB_disable_fext_ready] >>
+    last_assum (mp_tac o is_mem_do_nothing `SUC t`) >> rw []) >>
+  METIS_TAC [agp32_Rel_ag32_fext_MEM_correct_WB_not_NONE_WB_disable_fext_not_ready_extra]
+QED
+
+(** WB is not NONE and fext is not ready **)
+Theorem agp32_Rel_ag32_fext_MEM_correct_WB_not_NONE_extra:
+  !fext fbits a t I.
+    is_mem fext_accessor_circuit (agp32 fext fbits) fext ==>
+    is_sch I (agp32 fext fbits) a ==>
+    Rel I (fext t) (agp32 fext fbits (t-1)) (agp32 fext fbits t) a t ==>
+    I (5,SUC t) <> NONE ==>
+    ~(fext (SUC t)).ready ==>
+    (fext (SUC t)).mem = (FUNPOW Next (THE (I (5,SUC t)) - 1) a).MEM
+Proof
+  rw [] >> Cases_on `enable_stg 5 (agp32 fext fbits t)` >-
+   METIS_TAC [agp32_Rel_ag32_fext_MEM_correct_WB_not_NONE_WB_enable_extra] >>
+  METIS_TAC [agp32_Rel_ag32_fext_MEM_correct_WB_not_NONE_WB_disable_extra]
+QED
+
+
+(** mem is unchanged when WB is NONE **)
+Theorem agp32_mem_unchanged_when_WB_NONE:
+  !fext fbits a t I.
+    is_mem fext_accessor_circuit (agp32 fext fbits) fext ==>
+    is_sch I (agp32 fext fbits) a ==>
+    Rel I (fext t) (agp32 fext fbits (t-1)) (agp32 fext fbits t) a t ==>
+    I (5,SUC t) = NONE ==>
+    (fext (SUC t)).mem = (fext t).mem
+Proof
+  rw [] >> Cases_on `enable_stg 5 (agp32 fext fbits t)` >-
+   (`(fext t).ready` by (fs [enable_stg_def] >> METIS_TAC [agp32_WB_state_flag_and_fext_ready]) >>
+    `(agp32 fext fbits (SUC t)).WB.WB_opc = 16w \/ (agp32 fext fbits (SUC t)).WB.WB_opc = 15w`
+      by METIS_TAC [WB_instr_index_NONE_opc_flush] >>
+    `(agp32 fext fbits (SUC t)).command = 1w`
+      by METIS_TAC [agp32_Rel_ag32_command_correct_none_instr_WB_enable] >>
+    last_assum (assume_tac o is_mem_def_mem_no_errors) >>
+    last_assum (mp_tac o is_mem_inst_read `SUC t`) >> rw [] >>
+    Cases_on `m` >> fs [] >>
+    `(fext (0 + SUC t)).mem = (fext t).mem` by fs [] >> fs []) >>
+  Cases_on `(fext t).ready` >-
+   (`(agp32 fext fbits (SUC t)).command = 1w \/ (agp32 fext fbits (SUC t)).command = 0w`
+      by METIS_TAC [agp32_Rel_ag32_command_correct_WB_disable_fext_ready_extra] >>
+    last_assum (assume_tac o is_mem_def_mem_no_errors) >-
+     (last_assum (mp_tac o is_mem_inst_read `SUC t`) >> rw [] >>
+      Cases_on `m` >> fs [] >>
+      `(fext (0 + SUC t)).mem = (fext t).mem` by fs [] >> fs []) >>
+    last_assum (mp_tac o is_mem_do_nothing `SUC t`) >> rw []) >>
+  Cases_on `MAX_SET {t0 | t0 < t /\ (fext t0).ready}` >-
+   (last_assum (assume_tac o is_mem_def_mem_no_errors) >>
+    `(agp32 fext fbits (SUC 0)).command = 1w \/ (agp32 fext fbits (SUC 0)).command = 0w`
+      by METIS_TAC [agp32_command_cycle_1] >-
+     (last_assum (mp_tac o is_mem_inst_read `SUC 0`) >> simp [] >> strip_tac >>
+      Cases_on `~(fext (SUC t)).ready` >-
+       METIS_TAC [same_mem_t_SUC_t_under_MAX_SET_0] >> fs [ADD1] >>
+      `m = t` by METIS_TAC [same_t_and_m_under_MAX_SET_0] >> rw [] >>
+      Cases_on `m` >> gs [ADD1]) >>
+    last_assum (mp_tac o is_mem_do_nothing_spec `SUC 0`) >> simp [] >> strip_tac >>
+    Cases_on `(fext 0 ).ready` >> fs [] >-
+     (`!p. p < 0 ==> ~(fext (p + 1)).ready /\ (fext 0).mem = (fext (p + 1)).mem` by rw [] >>
+      `1 = 0 + 1` by rw [] >>
+      `(fext (0 + 1)).ready` by METIS_TAC [] >>
+      Cases_on `(fext (SUC t)).ready` >-
+       (`SUC t = t + 1` by rw [] >>
+        `0 = t` by METIS_TAC [same_t_and_m_under_MAX_SET_0] >> fs []) >>
+      METIS_TAC [same_mem_t_SUC_t_under_MAX_SET_0]) >>
+    `(!p. p < m + n' ==> ~(fext (p + 1)).ready)` by METIS_TAC [not_ready_m_plus_n] >>
+    `(!p. p < m ==> ~(fext (p + (n'+1))).ready)` by fs [] >>
+    Cases_on `(fext (SUC t)).ready` >-
+     (`SUC t = t + 1` by rw [] >>
+      FULL_SIMP_TAC std_ss [ADD_ASSOC] >>
+      `m + n' = t` by METIS_TAC [same_t_and_m_under_MAX_SET_0] >>
+      Q.ABBREV_TAC `m' = m + n'` >>
+      Cases_on `m` >> fs [] >>
+      `(fext (n' + (n + 1))).mem = (fext n').mem` by fs [] >>
+      `n' + (n + 1) = t` by fs [ADD1] >> fs []) >>
+    `(!p. p < m + n' ==> (fext (p + 1)).mem = (fext 0).mem)` by METIS_TAC [not_ready_m_plus_n_mem_0] >>
+    `(fext (m + n' + 1)).ready` by fs [] >>
+    METIS_TAC [same_mem_t_SUC_t_under_MAX_SET_0]) >>
+  Q.ABBREV_TAC `i = SUC n` >> `i <> 0` by fs [Abbr `i`] >>
+  `FINITE {t0 | t0 < t /\ (fext t0).ready}` by fs [FINITE_max_ready_cycle] >>
+  Cases_on `{t0 | t0 < t /\ (fext t0).ready} = {}` >> fs [MAX_SET_DEF] >>
+  `i IN {t0 | t0 < t /\ (fext t0).ready}` by METIS_TAC [MAX_SET_DEF] >> fs [MAX_SET_DEF] >>
+  last_assum (assume_tac o is_mem_def_mem_no_errors) >>
+  Cases_on_word_value `(agp32 fext fbits (SUC i)).command` >>
+  fs [agp32_command_impossible_values] >-
+   (last_assum (mp_tac o is_mem_data_flush `SUC i`) >> simp [] >> strip_tac >>
+    Cases_on `~(fext (SUC t)).ready` >-
+     METIS_TAC [same_mem_t_SUC_t_under_MAX_SET] >> fs [] >>
+    `m + SUC i = SUC t` by METIS_TAC [same_t_and_m_under_MAX_SET_SUC] >> fs [] >>
+    `(fext (m - 1 + SUC i)).mem = (fext i).mem` by fs [] >>
+    `m - 1 + SUC i = t` by fs [] >> fs []) >-
+   (last_assum (mp_tac o is_mem_data_write `SUC i`) >> simp [] >> strip_tac >>
+    Cases_on `~(fext (SUC t)).ready` >-
+     METIS_TAC [same_mem_t_SUC_t_under_MAX_SET] >> fs [] >>
+    `m + SUC i = SUC t` by METIS_TAC [same_t_and_m_under_MAX_SET_SUC] >> fs [] >>
+    Cases_on `enable_stg 5 (agp32 fext fbits i)` >-
+     (`(agp32 fext fbits (SUC i)).WB.WB_opc = (agp32 fext fbits (SUC t)).WB.WB_opc`
+        by METIS_TAC [WB_opc_unchanged_after_disabled_cycles] >>
+      `(agp32 fext fbits (SUC t)).WB.WB_opc = 16w \/ (agp32 fext fbits (SUC t)).WB.WB_opc = 15w`
+        by METIS_TAC [WB_instr_index_NONE_opc_flush] >>
+       gs [agp32_Rel_ag32_command_correct_none_instr_WB_enable]) >>
+    `(agp32 fext fbits (SUC i)).command = 0w \/ (agp32 fext fbits (SUC i)).command = 1w`
+      by METIS_TAC [agp32_Rel_ag32_command_correct_WB_disable_fext_ready_extra] >> fs []) >-
+   (last_assum (mp_tac o is_mem_data_read `SUC i`) >> simp [] >> strip_tac >>
+    Cases_on `~(fext (SUC t)).ready` >-
+     METIS_TAC [same_mem_t_SUC_t_under_MAX_SET] >> fs [] >>
+    `m + SUC i = SUC t` by METIS_TAC [same_t_and_m_under_MAX_SET_SUC] >> fs [] >>
+    `(fext (m - 1 + SUC i)).mem = (fext i).mem` by fs [] >>
+    `m - 1 + SUC i = t` by fs [] >> fs []) >-
+   (last_assum (mp_tac o is_mem_inst_read `SUC i`) >> simp [] >> strip_tac >>
+    Cases_on `~(fext (SUC t)).ready` >-
+     METIS_TAC [same_mem_t_SUC_t_under_MAX_SET] >> fs [] >>
+    `m + SUC i = SUC t` by METIS_TAC [same_t_and_m_under_MAX_SET_SUC] >> fs [] >>
+    `(fext (m - 1 + SUC i)).mem = (fext i).mem` by fs [] >>
+    `m - 1 + SUC i = t` by fs [] >> fs []) >>
+  last_assum (mp_tac o is_mem_do_nothing `SUC i`) >> simp [] >> strip_tac >>
+  Cases_on `SUC i = t` >> fs [] >>
+  Cases_on `SUC i > t` >> fs [] >>
+  `SUC i < t` by fs [] >>
+  `(SUC i) IN {t0 | t0 < t /\ (fext t0).ready}` by fs [] >>
+  `(SUC i) <= i` by METIS_TAC [MAX_SET_DEF] >> fs []
+QED
+
+
+(** MEM **)
+Theorem agp32_Rel_ag32_fext_MEM_correct_MEM_not_NONE:
+  !fext fbits a t I.
+    is_mem fext_accessor_circuit (agp32 fext fbits) fext ==>
+    is_sch I (agp32 fext fbits) a ==>
+    Rel I (fext t) (agp32 fext fbits (t-1)) (agp32 fext fbits t) a t ==>
+    I (5,SUC t) = NONE ==>
+    I (4,SUC t) <> NONE ==>
+    (fext (SUC t)).mem = (FUNPOW Next (THE (I (4,SUC t)) - 1) a).MEM
+Proof
+  rw [] >>
+  `(fext (SUC t)).mem = (fext t).mem` by METIS_TAC [agp32_mem_unchanged_when_WB_NONE] >>
+  Cases_on `enable_stg 4 (agp32 fext fbits t)` >-
+   (Cases_on `isMemOp_hw_op (agp32 fext fbits t)` >-
+     gs [is_sch_def,is_sch_memory_def] >>
+    `I' (4,SUC t) = I' (3,t)` by fs [is_sch_def,is_sch_memory_def] >>
+    `enable_stg 5 (agp32 fext fbits t)`
+      by fs [enable_stg_def,agp32_MEM_state_flag_eq_WB_state_flag] >>
+    `I' (5,SUC t) = I' (4,t)` by gs [is_sch_def,is_sch_writeback_def] >>
+    Cases_on `I' (5,t) = NONE` >> fs [Rel_def] >>
+    `(fext t).ready` by (fs [enable_stg_def] >> METIS_TAC [agp32_WB_state_flag_and_fext_ready]) >>
+    `THE (I' (3,t)) = THE (I' (5,t)) + 1`
+      by METIS_TAC [EX_instr_index_with_WB_instr_plus_1_MEM_NONE] >> fs []) >>
+  `~enable_stg 5 (agp32 fext fbits t)`
+    by fs [enable_stg_def,agp32_MEM_state_flag_eq_WB_state_flag] >>
+  `I' (5,SUC t) = I' (5,t) /\ I' (4,SUC t) = I' (4,t)` by gs [is_sch_def,is_sch_disable_def] >>
+  fs [Rel_def]
+QED
+
+(** EX **)
+Theorem agp32_Rel_ag32_fext_MEM_correct_EX_not_NONE:
+  !fext fbits a t I.
+    is_mem fext_accessor_circuit (agp32 fext fbits) fext ==>
+    is_sch I (agp32 fext fbits) a ==>
+    Rel I (fext t) (agp32 fext fbits (t-1)) (agp32 fext fbits t) a t ==>
+    I (5,SUC t) = NONE ==>
+    I (4,SUC t) = NONE ==>
+    I (3,SUC t) <> NONE ==>
+    (fext (SUC t)).mem = (FUNPOW Next (THE (I (3,SUC t)) - 1) a).MEM
+Proof
+  rw [] >>
+  `(fext (SUC t)).mem = (fext t).mem` by METIS_TAC [agp32_mem_unchanged_when_WB_NONE] >>
+  Cases_on `enable_stg 3 (agp32 fext fbits t)` >-
+   (Cases_on `isJump_hw_op (agp32 fext fbits t)` >-
+     gs [is_sch_def,is_sch_execute_def] >>
+    Cases_on `reg_data_hazard (agp32 fext fbits t)` >-
+     gs [is_sch_def,is_sch_execute_def] >>
+    `I' (3,SUC t) = I' (2,t)` by fs [is_sch_def,is_sch_execute_def] >>
+    `enable_stg 5 (agp32 fext fbits t)`
+      by fs [enable_stg_def,agp32_ID_EX_write_enable_WB_state_flag] >>
+    `I' (5,SUC t) = I' (4,t)` by gs [is_sch_def,is_sch_writeback_def] >>
+    `enable_stg 4 (agp32 fext fbits t)`
+      by fs [enable_stg_def,agp32_ID_EX_write_enable_MEM_state_flag] >>
+    Cases_on `isMemOp_hw_op (agp32 fext fbits t)` >-
+     (fs [enable_stg_def] >>
+      METIS_TAC [agp32_ID_EX_write_enable_no_MEM_stg_op]) >>
+    `I' (4,SUC t) = I' (3,t)` by METIS_TAC [is_sch_def,is_sch_memory_def] >> fs [] >>
+    Cases_on `I' (5,t) = NONE` >> fs [Rel_def] >>
+    `(fext t).ready` by (fs [enable_stg_def] >> METIS_TAC [agp32_WB_state_flag_and_fext_ready]) >>
+    `THE (I' (2,t)) = THE (I' (5,t)) + 1`
+      by METIS_TAC [EX_MEM_NONE_ID_instr_index_with_WB_instr_plus_1] >> fs []) >>
+  Cases_on `enable_stg 5 (agp32 fext fbits t)` >-
+   (`I' (3,SUC t) = I' (3,t)` by fs [is_sch_def,is_sch_disable_def] >> fs [] >>
+    `enable_stg 4 (agp32 fext fbits t)`
+      by fs [enable_stg_def,agp32_MEM_state_flag_eq_WB_state_flag] >>
+    Cases_on `isMemOp_hw_op (agp32 fext fbits t)` >-
+     (`I' (5,SUC t) = I' (4,t)` by gs [is_sch_def,is_sch_writeback_def] >> fs [] >>
+      Cases_on `I' (5,t) = NONE` >> fs [Rel_def] >>
+      `(fext t).ready` by (fs [enable_stg_def] >> METIS_TAC [agp32_WB_state_flag_and_fext_ready]) >>
+      `THE (I' (3,t)) = THE (I' (5,t)) + 1`
+        by METIS_TAC [EX_instr_index_with_WB_instr_plus_1_MEM_NONE] >> fs []) >>
+    fs [is_sch_def,is_sch_memory_def] >> METIS_TAC []) >>
+  `~enable_stg 4 (agp32 fext fbits t)`
+    by fs [enable_stg_def,agp32_MEM_state_flag_eq_WB_state_flag] >>
+  gs [is_sch_def,is_sch_disable_def,Rel_def]
+QED
+
+(** ID **)
+Theorem agp32_Rel_ag32_fext_MEM_correct_ID_not_NONE:
+  !fext fbits a t I.
+    is_mem fext_accessor_circuit (agp32 fext fbits) fext ==>
+    is_sch I (agp32 fext fbits) a ==>
+    Rel I (fext t) (agp32 fext fbits (t-1)) (agp32 fext fbits t) a t ==>
+    I (5,SUC t) = NONE ==>
+    I (4,SUC t) = NONE ==>
+    I (3,SUC t) = NONE ==>
+    I (2,SUC t) <> NONE ==>
+    (fext (SUC t)).mem = (FUNPOW Next (THE (I (2,SUC t)) - 1) a).MEM
+Proof
+  rw [] >>
+  `(fext (SUC t)).mem = (fext t).mem` by METIS_TAC [agp32_mem_unchanged_when_WB_NONE] >>
+  Cases_on `enable_stg 2 (agp32 fext fbits t)` >-
+   (Cases_on `isJump_isa_op (I' (2,t)) a \/ isJump_hw_op (agp32 fext fbits t)` >-
+     gs [is_sch_def,is_sch_decode_def] >>
+    `I' (2,SUC t) = I' (1,t)` by fs [is_sch_def,is_sch_decode_def] >> fs [] >>
+    `enable_stg 5 (agp32 fext fbits t)`
+      by fs [enable_stg_def,agp32_ID_ID_write_enable_WB_state_flag] >>
+    `I' (5,SUC t) = I' (4,t)` by gs [is_sch_def,is_sch_writeback_def] >> fs [] >>
+    `enable_stg 4 (agp32 fext fbits t)`
+      by fs [enable_stg_def,agp32_ID_ID_write_enable_MEM_state_flag] >>
+    Cases_on `isMemOp_hw_op (agp32 fext fbits t)` >-
+     (`enable_stg 3 (agp32 fext fbits t)`
+        by fs [enable_stg_def, agp32_ID_ID_write_enable_and_ID_EX_write_enable] >>
+      Cases_on `reg_data_hazard (agp32 fext fbits t)` >-
+       (fs [isJump_hw_op_def,enable_stg_def] >>
+        METIS_TAC [agp32_ID_ID_write_enable_EX_jump_sel_then_no_reg_data_hazard]) >>
+      `I' (3,SUC t) = I' (2,t)` by gs [is_sch_def,is_sch_execute_def] >> fs [] >>
+      `I' (3,t) = NONE` by METIS_TAC [IF_instr_NOT_NONE_ID_NONE_THEN_EX_NONE] >>
+      Cases_on `I' (5,t) = NONE` >> fs [Rel_def]) >>
+    `I' (4,SUC t) = I' (3,t)` by gs [is_sch_def,is_sch_memory_def] >> fs [] >>
+    `enable_stg 3 (agp32 fext fbits t)`
+      by fs [enable_stg_def,agp32_ID_ID_write_enable_and_ID_EX_write_enable] >>
+    Cases_on `reg_data_hazard (agp32 fext fbits t)` >-
+     (fs [isJump_hw_op_def,enable_stg_def] >>
+      METIS_TAC [agp32_ID_ID_write_enable_EX_jump_sel_then_no_reg_data_hazard]) >>
+    `I' (3,SUC t) = I' (2,t)` by gs [is_sch_def,is_sch_execute_def] >> fs [] >>
+    Cases_on `I' (5,t) = NONE` >> fs [Rel_def] >>
+    `THE (I' (1,t)) > THE (I' (5,t)) /\ THE (I' (1,t)) < THE (I' (5,t)) + 2`
+      by fs [Inv_Rel_def] >>
+    `THE (I' (1,t)) = THE (I' (5,t)) + 1` by fs [] >> fs []) >>
+  Cases_on `enable_stg 5 (agp32 fext fbits t)` >-
+   (`I' (5,SUC t) = I' (4,t)` by gs [is_sch_def,is_sch_writeback_def] >>
+    Cases_on `~enable_stg 3 (agp32 fext fbits t)` >> fs [] >-
+     (`I' (2,SUC t) = I' (2,t) /\ I' (3,SUC t) = I' (3,t)`
+        by METIS_TAC [is_sch_def,is_sch_disable_def] >> fs [] >>
+      Cases_on `I' (5,t) = NONE` >> fs [Rel_def] >>
+      `(fext t).ready` by (fs [enable_stg_def] >> METIS_TAC [agp32_WB_state_flag_and_fext_ready]) >>
+      `THE (I' (2,t)) = THE (I' (5,t)) + 1`
+        by METIS_TAC [EX_MEM_NONE_ID_instr_index_with_WB_instr_plus_1] >> fs []) >>
+    `I' (2,SUC t) = I' (2,t)` by METIS_TAC [is_sch_def,is_sch_disable_def] >> fs [] >>
+    `enable_stg 4 (agp32 fext fbits t)`
+      by fs [enable_stg_def,agp32_MEM_state_flag_eq_WB_state_flag] >>
+    `~isMemOp_hw_op (agp32 fext fbits t)`
+      by fs [enable_stg_def,agp32_ID_EX_write_enable_no_MEM_stg_op] >>
+    `I' (4,SUC t) = I' (3,t)` by METIS_TAC [is_sch_def,is_sch_memory_def] >> fs [] >>
+    Cases_on `I' (5,t) = NONE` >> fs [Rel_def] >>
+    `(fext t).ready` by (fs [enable_stg_def] >> METIS_TAC [agp32_WB_state_flag_and_fext_ready]) >>
+    `THE (I' (2,t)) = THE (I' (5,t)) + 1`
+      by METIS_TAC [EX_MEM_NONE_ID_instr_index_with_WB_instr_plus_1] >> fs []) >>
+  Cases_on `enable_stg 4 (agp32 fext fbits t)` >-
+   (fs [enable_stg_def] >> fs [agp32_MEM_state_flag_eq_WB_state_flag]) >>
+  `~enable_stg 3 (agp32 fext fbits t)`
+    by fs [enable_stg_def,agp32_MEM_state_flag_F_and_ID_EX_write_disable] >>
+  gs [is_sch_def,is_sch_disable_def,Rel_def]
+QED
+
+(** IF **)
+Theorem agp32_Rel_ag32_fext_MEM_correct_IF_not_NONE:
+  !fext fbits a t I.
+    is_mem fext_accessor_circuit (agp32 fext fbits) fext ==>
+    is_sch I (agp32 fext fbits) a ==>
+    Rel I (fext t) (agp32 fext fbits (t-1)) (agp32 fext fbits t) a t ==>
+    I (5,SUC t) = NONE ==>
+    I (4,SUC t) = NONE ==>
+    I (3,SUC t) = NONE ==>
+    I (2,SUC t) = NONE ==>
+    I (1,SUC t) <> NONE ==>
+    (fext (SUC t)).mem = (FUNPOW Next (THE (I (1,SUC t)) - 1) a).MEM
+Proof
+  rw [] >>
+  `(fext (SUC t)).mem = (fext t).mem` by METIS_TAC [agp32_mem_unchanged_when_WB_NONE] >>
+  Cases_on `enable_stg 1 (agp32 fext fbits t)` >-
+   (Cases_on `isJump_hw_op (agp32 fext fbits t)` >-
+     (`I' (1,SUC t) = SOME (THE (I' (3,t)) + 1)` by fs [is_sch_def,is_sch_fetch_def] >>
+      `isJump_isa_op (I' (3,t)) a` by fs [Rel_def,EX_Rel_spec_def,isJump_hw_op_def] >>
+      `I' (3,t) <> NONE` by METIS_TAC [isJump_isa_op_not_none] >>
+      `enable_stg 4 (agp32 fext fbits t)`
+        by fs [enable_stg_def,agp32_IF_PC_write_enable_and_MEM_flag] >>
+      `enable_stg 3 (agp32 fext fbits t)`
+        by fs [enable_stg_def,agp32_IF_PC_write_enable_and_ID_EX_write_enable] >>
+      Cases_on `isMemOp_hw_op (agp32 fext fbits t)` >-
+       (fs [enable_stg_def] >>    
+        METIS_TAC [MEM_stg_op_agp32_ID_EX_write_disable]) >>
+      `I' (4,SUC t) = I' (3,t)` by gs [is_sch_def,is_sch_memory_def] >> fs []) >>
+    Cases_on `isJump_isa_op (I' (1,t)) a \/ isJump_isa_op (I' (2,t)) a \/ I' (1,t) = NONE` >-
+     gs [is_sch_def,is_sch_fetch_def,is_sch_execute_def] >>
+    `enable_stg 2 (agp32 fext fbits t)`
+      by fs [enable_stg_def,agp32_IF_PC_write_enable_and_ID_ID_write_enable] >>
+    `I' (2,SUC t) = I' (1,t)` by METIS_TAC [is_sch_def,is_sch_decode_def] >> fs []) >>
+  `~enable_stg 2 (agp32 fext fbits t)`
+    by METIS_TAC [enable_stg_def,agp32_IF_PC_write_enable_and_ID_ID_write_enable] >>
+  Cases_on `enable_stg 5 (agp32 fext fbits t)` >-
+   (`I' (5,SUC t) = I' (4,t)` by gs [is_sch_def,is_sch_writeback_def] >>
+    Cases_on `~enable_stg 3 (agp32 fext fbits t)` >> fs [] >-
+     (`I' (1,SUC t) = I' (1,t) /\ I' (2,SUC t) = I' (2,t) /\ I' (3,SUC t) = I' (3,t)`
+        by gs [is_sch_def,is_sch_disable_def] >> fs [] >>
+      Cases_on `I' (5,t) = NONE` >> fs [Rel_def] >>
+      `(fext t).ready` by (fs [enable_stg_def] >> METIS_TAC [agp32_WB_state_flag_and_fext_ready]) >>
+      `THE (I' (1,t)) = THE (I' (5,t)) + 1` by fs [Inv_Rel_def] >> fs []) >>
+    `enable_stg 4 (agp32 fext fbits t)`
+      by fs [enable_stg_def,agp32_MEM_state_flag_eq_WB_state_flag] >>
+    `~isMemOp_hw_op (agp32 fext fbits t)`
+      by fs [enable_stg_def,agp32_ID_EX_write_enable_no_MEM_stg_op] >>
+    `I' (4,SUC t) = I' (3,t)` by METIS_TAC [is_sch_def,is_sch_memory_def] >> fs [] >>
+    `I' (1,SUC t) = I' (1,t) /\ I' (2,SUC t) = I' (2,t)`
+      by METIS_TAC [is_sch_def,is_sch_disable_def] >> fs [] >>
+    Cases_on `I' (5,t) = NONE` >> fs [Rel_def] >>
+    `(fext t).ready` by (fs [enable_stg_def] >> METIS_TAC [agp32_WB_state_flag_and_fext_ready]) >>
+    `THE (I' (1,t)) = THE (I' (5,t)) + 1` by fs [Inv_Rel_def] >> fs []) >>
+  `~enable_stg 4 (agp32 fext fbits t)` by fs [enable_stg_def,agp32_MEM_state_flag_eq_WB_state_flag] >>
+  `~enable_stg 3 (agp32 fext fbits t)`
+    by fs [enable_stg_def,agp32_MEM_state_flag_F_and_ID_EX_write_disable] >>
+  gs [is_sch_def,is_sch_disable_def,Rel_def]
 QED
 
 
